backend/Linear.v
@@ -48,8 +48,7 @@ Record function: Type := mkfunction {
   fn_code: code
 }.
 
-#[global]
-Instance has_comp_function: has_comp function := fn_comp.
+#[global] Instance has_comp_function: has_comp function := fn_comp.
 
 Definition fundef := AST.fundef function.
 
