riscV/Asmgenproof.v
@@ -71,7 +71,7 @@ Qed.
 
 Lemma find_comp_translated:
   forall vf,
-    Genv.find_comp ge vf = Genv.find_comp tge vf.
+    Genv.find_comp_in_genv ge vf = Genv.find_comp_in_genv tge vf.
 Proof.
   eapply (Genv.find_comp_transf_partial TRANSF).
 Qed.
@@ -107,12 +107,15 @@ Proof.
 Qed.
 
 Lemma exec_straight_exec:
-  forall fb f c ep tf tc c' rs m rs' m' st,
+  forall fb f c ep tf tc c' rs m rs' m' st cp,
   transl_code_at_pc ge (rs PC) fb f c ep tf tc ->
   exec_straight tge tf tc rs m c' rs' m' ->
-  plus step tge (State st rs m) E0 (State st rs' m').
+  cp = Genv.find_comp_in_genv ge (rs PC) ->
+  plus step tge (State st rs m cp) E0 (State st rs' m' cp).
 Proof.
   intros. inv H.
+  rewrite <- H2; simpl; erewrite Genv.find_funct_ptr_find_comp_of_block; eauto; simpl;
+    rewrite comp_transf_function; eauto.
   eapply exec_straight_steps_1; eauto.
   eapply transf_function_no_overflow; eauto.
   eapply functions_transl; eauto.
@@ -525,15 +528,15 @@ Inductive match_stacks cp : list Mach.stackframe -> stack -> Prop :=
     (* Intra-compartment calls create a new frame in the source, but not the target *)
     forall s s' f,
     match_stacks cp s s' ->
-    Mach.call_comp ge (f :: s) = Some cp -> (* meaning, we are staying in the same
+    Mach.call_comp ge (f :: s) = cp -> (* meaning, we are staying in the same
                                                compartment *)
     match_stacks cp (f :: s) s'
 | match_stacks_cross_compartment:
     (* Cross-compartment calls create a new frame in both the source and the target *)
     forall cp' s s' f f',
     match_stacks cp' s s' ->
-    Mach.call_comp ge (f :: s) = Some cp' ->
-    call_comp tge (f' :: s') = Some cp' ->
+    Mach.call_comp ge (f :: s) = cp' ->
+    call_comp tge (f' :: s') = cp' ->
     cp <> cp' ->
     match_stackframe f f' ->
     match_stacks cp (f :: s) (f' :: s')
@@ -550,18 +553,18 @@ Inductive match_states: Mach.state -> Asm.state -> Prop :=
         (AG: agree ms sp rs)
         (DXP: ep = true -> rs#X30 = parent_sp s),
       match_states (Mach.State s fb sp c ms m)
-                   (Asm.State s' rs m')
+        (Asm.State s' rs m' (comp_of f))
   | match_states_call:
-      forall s s' fb ms m m' rs sig cp
+      forall s s' fb ms m m' rs sig cp cp'
         (STACKS: match_stack ge s)
-        (STACKS_COMP: Genv.find_comp_of_block ge fb = Some cp)
+        (STACKS_COMP: Genv.find_comp_of_block ge fb = cp)
         (STACKS': match_stacks cp s s')
         (MEXT: Mem.extends m m')
         (AG: agree ms (parent_sp s) rs)
         (ATPC: rs PC = Vptr fb Ptrofs.zero)
         (ATLR: rs RA = parent_ra s),
-      match_states (Mach.Callstate s fb sig ms m)
-                   (Asm.State s' rs m')
+      match_states (Mach.Callstate s fb sig ms m cp')
+                   (Asm.State s' rs m' cp')
   | match_states_return:
     forall s s' ms m m' rs cp
       (STACKS: match_stack ge s)
@@ -585,13 +588,14 @@ Lemma exec_straight_steps:
     /\ agree ms2 sp rs2
     /\ (it1_is_parent ep i = true -> rs2#X30 = parent_sp s)) ->
   exists st',
-  plus step tge (State s' rs1 m1') E0 st' /\
+  plus step tge (State s' rs1 m1' (comp_of f)) E0 st' /\
   match_states (Mach.State s fb sp c ms2 m2) st'.
 Proof.
   intros. inversion H2. subst. monadInv H7.
   exploit H3; eauto. intros [rs2 [A [B C]]].
-  exists (State s' rs2 m2'); split.
+  exists (State s' rs2 m2' (comp_of f)); split.
   eapply exec_straight_exec; eauto.
+  now rewrite <- H4; simpl; erewrite Genv.find_funct_ptr_find_comp_of_block; eauto.
   econstructor; eauto.
   eapply exec_straight_at; eauto.
 Qed.
@@ -613,7 +617,7 @@ Lemma exec_straight_steps_goto:
     /\ sig_call jmp = None
     /\ is_return jmp = false) ->
   exists st',
-  plus step tge (State s' rs1 m1') E0 st' /\
+  plus step tge (State s' rs1 m1' (comp_of f)) E0 st' /\
   match_states (Mach.State s fb sp c' ms2 m2) st'.
 Proof.
   intros. inversion H3. subst. monadInv H9.
@@ -625,16 +629,17 @@ Proof.
   exploit find_label_goto_label; eauto.
   intros [tc' [rs3 [GOTO [AT' OTH]]]].
   inversion AT'; subst.
-  exists (State s' rs3 m2'); split.
+  exists (State s' rs3 m2' (comp_of f)); split.
   eapply plus_right'.
-  eapply exec_straight_steps_1; eauto. unfold Genv.find_comp.
-  { econstructor. eauto. eauto.
+  rewrite comp_transf_function; eauto.
+  eapply exec_straight_steps_1; eauto.
+  { rewrite comp_transf_function; eauto.
+    econstructor. eauto. eauto.
     eapply find_instr_tail. eauto.
     rewrite <- comp_transf_function; eauto.
     rewrite C. eexact GOTO. auto. auto.
     eauto.
-    simpl. now rewrite (Genv.find_funct_ptr_find_comp_of_block _ _ FN).
-  }
+    simpl. now rewrite (Genv.find_funct_ptr_find_comp_of_block _ _ FN). }
   traceEq.
   econstructor; eauto.
   apply agree_exten with rs2; auto with asmgen.
@@ -658,7 +663,7 @@ Lemma exec_straight_opt_steps_goto:
     /\ sig_call jmp = None
     /\ is_return jmp = false) ->
   exists st',
-  plus step tge (State s' rs1 m1') E0 st' /\
+  plus step tge (State s' rs1 m1' (comp_of f)) E0 st' /\
   match_states (Mach.State s fb sp c' ms2 m2) st'.
 Proof.
   intros. inversion H3. subst. monadInv H9.
@@ -669,9 +674,10 @@ Proof.
 - exploit find_label_goto_label; eauto.
   intros [tc' [rs3 [GOTO [AT' OTH]]]].
   inversion AT'; subst.
-  exists (State s' rs3 m2'); split.
+  exists (State s' rs3 m2' (comp_of f)); split.
   apply plus_one.
-  { econstructor. eauto. eauto.
+  { rewrite comp_transf_function; eauto.
+    econstructor. eauto. eauto.
     eapply find_instr_tail. eauto.
     rewrite C. eexact GOTO. auto. auto.
     eauto. simpl. now rewrite (Genv.find_funct_ptr_find_comp_of_block _ _ FN).
@@ -684,10 +690,12 @@ Proof.
   exploit find_label_goto_label; eauto.
   intros [tc' [rs3 [GOTO [AT' OTH]]]].
   inversion AT'; subst.
-  exists (State s' rs3 m2'); split.
+  exists (State s' rs3 m2' (comp_of f)); split.
   eapply plus_right'.
+  rewrite comp_transf_function; eauto.
   eapply exec_straight_steps_1; eauto.
-  { econstructor. eauto. eauto.
+  { rewrite comp_transf_function; eauto.
+    econstructor. eauto. eauto.
     eapply find_instr_tail. eauto.
     rewrite C. eexact GOTO. auto. auto.
     eauto. simpl. now rewrite (Genv.find_funct_ptr_find_comp_of_block _ _ FN).
@@ -709,7 +717,7 @@ Qed.
 Definition measure (s: Mach.state) : nat :=
   match s with
   | Mach.State _ _ _ _ _ _ => 0%nat
-  | Mach.Callstate _ _ _ _ _ => 2%nat
+  | Mach.Callstate _ _ _ _ _ _ => 2%nat
   | Mach.Returnstate _ _ _ _ => 1%nat
   end.
 
@@ -719,7 +727,7 @@ Proof.
   exploit preg_of_injective; eauto. intros; subst r; discriminate.
 Qed.
 
-Ltac unfold_find_comp A R :=
+Ltac unfold_find_comp_in_genv A R :=
   rewrite (Genv.find_funct_ptr_find_comp_of_block _ _ R) in A;
   injection A as A.
 
@@ -744,8 +752,10 @@ Proof.
   rewrite (sp_val _ _ _ AG) in A.
   left; eapply exec_straight_steps; eauto. intros. simpl in TR.
   inv AT.
-  unfold_find_comp CURCOMP FIND.
-  rewrite <- CURCOMP in A. setoid_rewrite (comp_transf_function) in A; eauto.
+  (* unfold_find_comp_in_genv CURCOMP FIND. *)
+  unfold Genv.find_comp_of_block in A; unfold Genv.find_funct_ptr in FIND.
+    destruct (Genv.find_def ge f) as [[] |] eqn:?; try congruence. inv FIND. simpl in A.
+  setoid_rewrite (comp_transf_function) in A; eauto.
   exploit loadind_correct; eauto with asmgen. intros [rs' [P [Q R]]].
   exists rs'; split. eauto.
   split. eapply agree_set_mreg; eauto with asmgen. congruence.
@@ -758,8 +768,9 @@ Proof.
   left; eapply exec_straight_steps; eauto.
   rewrite (sp_val _ _ _ AG) in A. intros. simpl in TR.
   inv AT.
-  unfold_find_comp CURCOMP FIND.
-  setoid_rewrite <- CURCOMP in A. setoid_rewrite (comp_transf_function) in A; eauto.
+  unfold Genv.find_comp_of_block in A; unfold Genv.find_funct_ptr in FIND.
+    destruct (Genv.find_def ge f) as [[] |] eqn:?; try congruence. inv FIND. simpl in A.
+  setoid_rewrite (comp_transf_function) in A; eauto.
   exploit storeind_correct; eauto with asmgen. intros [rs' [P Q]].
   exists rs'; split. eauto.
   split. eapply agree_undef_regs; eauto with asmgen.
@@ -788,8 +799,9 @@ Opaque loadind.
 (* GPR11 does not contain parent *)
   rewrite chunk_of_Tptr in A.
   inv AT.
-  unfold_find_comp CURCOMP FIND.
-  setoid_rewrite <- CURCOMP in A. setoid_rewrite (comp_transf_function) in A; eauto.
+  unfold Genv.find_comp_of_block in A; unfold Genv.find_funct_ptr in FIND.
+    destruct (Genv.find_def ge fb) as [[] |] eqn:?; try congruence. inv FIND. simpl in A.
+  setoid_rewrite (comp_transf_function) in A; eauto.
   exploit loadind_ptr_correct. eexact A. congruence. intros [rs1 [P [Q R]]].
   exploit loadind_priv_correct. eexact EQ. instantiate (2 := rs1). rewrite Q. eauto. congruence.
   intros [rs2 [S [T U]]].
@@ -825,8 +837,9 @@ Local Transparent destroyed_by_op.
   exploit Mem.loadv_extends; eauto. intros [v' [C D]].
   left; eapply exec_straight_steps; eauto; intros. simpl in TR.
   inv AT.
-  unfold_find_comp CURCOMP FIND.
-  setoid_rewrite <- CURCOMP in C. setoid_rewrite (comp_transf_function) in C; eauto.
+  unfold Genv.find_comp_of_block in C; unfold Genv.find_funct_ptr in FIND.
+    destruct (Genv.find_def ge f) as [[] |] eqn:?; try congruence. inv FIND. simpl in C.
+  setoid_rewrite (comp_transf_function) in C; eauto.
   exploit transl_load_correct; eauto. intros [rs2 [P [Q R]]].
   exists rs2; split. eauto.
   split. eapply agree_set_undef_mreg; eauto. congruence.
@@ -842,8 +855,9 @@ Local Transparent destroyed_by_op.
   exploit Mem.storev_extends; eauto. intros [m2' [C D]].
   left; eapply exec_straight_steps; eauto.
   inv AT.
-  unfold_find_comp CURCOMP FIND.
-  setoid_rewrite <- CURCOMP in C. setoid_rewrite (comp_transf_function) in C; eauto.
+  unfold Genv.find_comp_of_block in C; unfold Genv.find_funct_ptr in FIND.
+    destruct (Genv.find_def ge f) as [[] |] eqn:?; try congruence. inv FIND. simpl in C.
+  setoid_rewrite (comp_transf_function) in C; eauto.
   intros. simpl in TR. exploit transl_store_correct; eauto. intros [rs2 [P Q]].
   exists rs2; split. eauto.
   split. eapply agree_undef_regs; eauto with asmgen.
@@ -870,9 +884,11 @@ Local Transparent destroyed_by_op.
   instantiate (1 := (rs0 # PC <- (rs0 x0)) # X1 <- (Val.offset_ptr (rs0 PC) Ptrofs.one)).
   simpl. eapply agree_exten. eapply agree_undef_regs; eauto. intros. Simpl.
   intros [args' [ARGS' LDARGS]].
-  destruct ((comp_of (Internal tf) =? comp_of tf')%positive) eqn:Heq.
+  destruct (cp_eq_dec (comp_of tf') (comp_of tf)) eqn:Heq.
   * left; econstructor; split.
-    apply plus_one. eapply exec_step_internal_call with (args := args').
+    apply plus_one.
+    rewrite comp_transf_function.
+    eapply exec_step_internal_call with (args := args').
     rewrite <- H2; simpl; eauto.
     eapply functions_transl; eauto.
     eapply find_instr_tail; eauto.
@@ -886,77 +902,177 @@ Local Transparent destroyed_by_op.
     rewrite H7; simpl.
     unfold tge.
     rewrite (Genv.find_funct_ptr_find_comp_of_block _ _ TFIND).
-    unfold comp_of in *; simpl in *; unfold comp_of in *; now rewrite Heq.
+    rewrite e; destruct (cp_eq_dec (comp_of tf) (comp_of tf)); try now auto.
     auto.
+    rewrite e, Genv.type_of_call_same_cp; now auto.
     (* Not a cross-compartment call *)
-    { unfold Genv.type_of_call; simpl in *.
-      unfold comp_of. unfold comp_of in Heq. now setoid_rewrite Heq. }
+    (* { destruct (cp_eq_dec (comp_of tf) (comp_of tf)); try now auto. } *)
+    (* pose proof (flowsto_refl (comp_of tf)); try now auto. } *)
     { rewrite <- comp_transf_function; eauto.
       rewrite <- (comp_transl_partial _ TTRANSF); eauto.
       eapply call_trace_lessdef; eauto using senv_preserved, symbols_preserved. }
+    eauto.
+    (* replace (comp_of f) with (comp_of tf'). *)
+    (* replace (comp_of f) with (Genv.find_comp_in_genv ge (Vptr fb (Ptrofs.add ofs Ptrofs.one))). *)
+    rewrite comp_transf_function; eauto.
     econstructor; eauto.
     econstructor; eauto.
     eapply agree_sp_def; eauto.
-    { rewrite find_comp_of_block_translated. unfold tge.
-      now rewrite (Genv.find_funct_ptr_find_comp_of_block _ _ TFIND). }
+    (* { rewrite find_comp_translated. unfold tge. *)
+    (*   unfold Genv.find_comp_in_genv. simpl. *)
+    (*   exploit functions_transl; eauto. intros G. *)
+    (*   rewrite (Genv.find_funct_ptr_find_comp_of_block _ _ G). *)
+    (*   rewrite comp_transf_function; simpl; eauto. } *)
     { Simpl.
       change (comp_of (Internal tf)) with (comp_of tf) in Heq.
-      apply Peqb_true_eq in Heq. rewrite <- Heq.
-      rewrite <- (comp_transf_function _ _ H4).
+      rewrite (Genv.find_funct_ptr_find_comp_of_block _ _ CALLED).
       apply match_stacks_intra_compartment; trivial.
+      replace (comp_of fd) with (comp_of f). auto.
+      { rewrite comp_transf_function; eauto.
+        unfold transf_fundef, transf_partial_fundef in TTRANSF.
+        destruct fd.
+        - monadInv TTRANSF. simpl in *.
+          rewrite comp_transf_function. rewrite e; eauto.
+          eauto.
+        - inv TTRANSF. simpl in *. auto. }
       unfold Mach.call_comp. simpl.
-      now rewrite (Genv.find_funct_ptr_find_comp_of_block _ _ FIND). }
-    simpl. eapply agree_exten; eauto. intros. Simpl.
-    Simpl. rewrite <- H2. auto.
-  * left; econstructor; split.
-    apply plus_one. eapply exec_step_internal_call.
-    rewrite <- H2; simpl; eauto.
-    eapply functions_transl; eauto.
-    eapply find_instr_tail; eauto.
-    simpl; eauto.
-    simpl; eauto.
-    Simpl; eauto.
-    rewrite <- (comp_transl_partial _ H4).
-    eapply allowed_call_translated; eauto.
-    simpl.
-    now rewrite (Genv.find_funct_ptr_find_comp_of_block _ _ TFIND).
-    unfold update_stack_call. Simpl.
-    rewrite H7; simpl.
-    simpl.
-    unfold tge; rewrite (Genv.find_funct_ptr_find_comp_of_block _ _ TFIND).
-    rewrite <- H2. simpl.
-    replace (comp_of tf =? comp_of tf')%positive with false.
-    reflexivity.
-    eauto.
-    { simpl.
-      intros.
-      rewrite <- (comp_transl_partial _ H4) in H8.
-      rewrite <- (comp_transl_partial _ TTRANSF) in H8.
-      specialize (NO_CROSS_PTR H8).
-      now eapply Val.lessdef_list_not_ptr; eauto. }
-    { simpl. rewrite <- comp_transf_function; eauto.
-      rewrite <- (comp_transl_partial _ TTRANSF).
-      eapply call_trace_lessdef; eauto using senv_preserved, symbols_preserved. }
-    econstructor; eauto.
-    econstructor; eauto.
-    eapply agree_sp_def; eauto.
-    { Simpl.
-      now rewrite (Genv.find_funct_ptr_find_comp_of_block _ _ CALLED). }
-    (* TODO: clean *)
-    { eapply match_stacks_cross_compartment. exact STACKS'.
-      - unfold Mach.call_comp. simpl.
-        now rewrite (Genv.find_funct_ptr_find_comp_of_block _ _ FIND).
-      - simpl.
-        rewrite <- find_comp_of_block_translated.
-        now rewrite (Genv.find_funct_ptr_find_comp_of_block _ _ H3).
-      - rewrite (comp_transl_partial _ TTRANSF).
-        rewrite (comp_transl_partial _ H4).
-        intros contra. now rewrite contra, Pos.eqb_refl in Heq.
-      - erewrite agree_sp; eauto.
-        constructor.
+      rewrite (Genv.find_funct_ptr_find_comp_of_block _ _ FIND).
+      { simpl.
+        rewrite comp_transf_function; eauto.
+        unfold transf_fundef, transf_partial_fundef in TTRANSF.
+        destruct fd.
+        - monadInv TTRANSF. simpl in *.
+          rewrite comp_transf_function. rewrite e; eauto.
+          eauto.
+        - inv TTRANSF. simpl in *. auto. }
     }
     simpl. eapply agree_exten; eauto. intros. Simpl.
     Simpl. rewrite <- H2. auto.
+    (* simpl. *)
+    (* now rewrite e, comp_transf_function. *)
+  * destruct (flowsto_dec (comp_of tf') (comp_of tf)) eqn:?.
+    -- left; econstructor; split.
+       rewrite comp_transf_function.
+       apply plus_one. eapply exec_step_internal_call.
+       rewrite <- H2; simpl; eauto.
+       eapply functions_transl; eauto.
+       eapply find_instr_tail; eauto.
+       simpl; eauto.
+       simpl; eauto.
+       Simpl; eauto.
+       rewrite <- (comp_transl_partial _ H4).
+       eapply allowed_call_translated; eauto.
+       simpl.
+       now rewrite (Genv.find_funct_ptr_find_comp_of_block _ _ TFIND).
+       unfold update_stack_call. Simpl.
+       rewrite H7; simpl.
+       simpl.
+       unfold tge; rewrite (Genv.find_funct_ptr_find_comp_of_block _ _ TFIND).
+       rewrite <- H2. simpl. rewrite Heq.
+       reflexivity.
+       eauto.
+       { simpl.
+         intros.
+         rewrite <- (comp_transl_partial _ H4) in H8.
+         rewrite <- (comp_transl_partial _ TTRANSF) in H8.
+         specialize (NO_CROSS_PTR H8).
+         now eapply Val.lessdef_list_not_ptr; eauto. }
+       { simpl. rewrite <- comp_transf_function; eauto.
+         rewrite <- (comp_transl_partial _ TTRANSF).
+         eapply call_trace_lessdef; eauto using senv_preserved, symbols_preserved. }
+       eauto.
+       (* replace (comp_of f) *)
+       (*   with (Genv.find_comp_in_genv ge (Vptr fb (Ptrofs.add ofs Ptrofs.one))). *)
+       rewrite comp_transf_function; eauto.
+       econstructor; eauto.
+       econstructor; eauto.
+       eapply agree_sp_def; eauto.
+       (* TODO: clean *)
+       { eapply match_stacks_cross_compartment. exact STACKS'.
+         - unfold Mach.call_comp. simpl.
+           now rewrite (Genv.find_funct_ptr_find_comp_of_block _ _ FIND).
+         - simpl.
+           rewrite <- find_comp_of_block_translated.
+           now rewrite (Genv.find_funct_ptr_find_comp_of_block _ _ H3).
+         - rewrite (Genv.find_funct_ptr_find_comp_of_block _ _ CALLED).
+           simpl.
+           rewrite comp_transf_function; eauto.
+           unfold transf_fundef, transf_partial_fundef in TTRANSF.
+           destruct fd.
+           + monadInv TTRANSF. simpl in *.
+             rewrite comp_transf_function; eauto.
+           + inv TTRANSF. simpl in *. auto.
+         - erewrite agree_sp; eauto.
+           constructor.
+       }
+       simpl. eapply agree_exten; eauto. intros. Simpl.
+       Simpl. rewrite <- H2. auto.
+       (* simpl. *)
+       (* now rewrite (Genv.find_funct_ptr_find_comp_of_block _ _ H3). *)
+    -- left; econstructor; split.
+       rewrite comp_transf_function; eauto.
+       apply plus_one. eapply exec_step_internal_call.
+       rewrite <- H2; simpl; eauto.
+       eapply functions_transl; eauto.
+       eapply find_instr_tail; eauto.
+       simpl; eauto.
+       simpl; eauto.
+       Simpl; eauto.
+       rewrite <- (comp_transl_partial _ H4).
+       eapply allowed_call_translated; eauto.
+       simpl.
+       now rewrite (Genv.find_funct_ptr_find_comp_of_block _ _ TFIND).
+       unfold update_stack_call. Simpl.
+       rewrite H7; simpl.
+       simpl.
+       unfold tge; rewrite (Genv.find_funct_ptr_find_comp_of_block _ _ TFIND).
+       rewrite <- H2. simpl. rewrite Heq.
+       reflexivity.
+       eauto.
+       { simpl.
+         intros.
+         rewrite <- (comp_transl_partial _ H4) in H8.
+         rewrite <- (comp_transl_partial _ TTRANSF) in H8.
+         specialize (NO_CROSS_PTR H8).
+         now eapply Val.lessdef_list_not_ptr; eauto. }
+       { simpl. rewrite <- comp_transf_function; eauto.
+         rewrite <- (comp_transl_partial _ TTRANSF).
+         eapply call_trace_lessdef; eauto using senv_preserved, symbols_preserved. }
+       (* replace (comp_of f) *)
+       (*   with (Genv.find_comp_in_genv ge (Vptr fb (Ptrofs.add ofs Ptrofs.one))). *)
+       rewrite comp_transf_function; eauto.
+       econstructor; eauto.
+       econstructor; eauto.
+       eapply agree_sp_def; eauto.
+       (* { rewrite find_comp_translated. unfold tge. *)
+       (*   unfold Genv.find_comp_in_genv. simpl. *)
+       (*   exploit functions_transl; eauto. intros G. *)
+       (*   rewrite (Genv.find_funct_ptr_find_comp_of_block _ _ G). *)
+       (*   rewrite comp_transf_function; simpl; eauto. } *)
+       (* TODO: clean *)
+       { eapply match_stacks_cross_compartment. exact STACKS'.
+         - unfold Mach.call_comp. simpl.
+           now rewrite (Genv.find_funct_ptr_find_comp_of_block _ _ FIND).
+         - simpl.
+           rewrite <- find_comp_of_block_translated.
+           now rewrite (Genv.find_funct_ptr_find_comp_of_block _ _ H3).
+         (* - rewrite (comp_transl_partial _ TTRANSF). *)
+         (*   rewrite (comp_transl_partial _ H4). *)
+         (*   intros contra. now rewrite contra, Pos.eqb_refl in Heq. *)
+         - rewrite (Genv.find_funct_ptr_find_comp_of_block _ _ CALLED).
+           simpl.
+           rewrite comp_transf_function; eauto.
+           unfold transf_fundef, transf_partial_fundef in TTRANSF.
+           destruct fd.
+           + monadInv TTRANSF. simpl in *.
+             rewrite comp_transf_function; eauto.
+           + inv TTRANSF. simpl in *. auto.
+         - erewrite agree_sp; eauto.
+           constructor.
+       }
+       simpl. eapply agree_exten; eauto. intros. Simpl.
+       Simpl. rewrite <- H2. auto.
+       (* simpl. now rewrite (Genv.find_funct_ptr_find_comp_of_block _ _ H3). *)
 + (* Direct call *)
   generalize (code_tail_next_int _ _ _ _ NOOV H6). intro CT1.
   assert (TCA: transl_code_at_pc ge (Vptr fb (Ptrofs.add ofs Ptrofs.one)) fb f c false tf x).
@@ -966,8 +1082,9 @@ Local Transparent destroyed_by_op.
   instantiate (1 := (rs0 # PC <- (Genv.symbol_address tge fid Ptrofs.zero)) # X1 <- (Val.offset_ptr (rs0 PC) Ptrofs.one)).
   simpl. eapply agree_exten. eapply agree_undef_regs; eauto. intros. Simpl.
   intros [args' [ARGS' LDARGS]].
-  destruct (comp_of (Internal tf) =? comp_of tf')%positive eqn:Heq.
+  destruct (cp_eq_dec (comp_of tf') (comp_of tf)) eqn:Heq.
   * left; econstructor; split.
+    rewrite comp_transf_function; eauto.
     apply plus_one. eapply exec_step_internal_call.
     rewrite <- H2; simpl; eauto.
     eapply functions_transl; eauto.
@@ -987,72 +1104,175 @@ Local Transparent destroyed_by_op.
     unfold comp_of in *; simpl in *. unfold comp_of in *. now rewrite Heq.
     eauto.
     (* Not a cross-compartment call *)
-    { unfold Genv.type_of_call; simpl in *.
-      unfold comp_of. unfold comp_of in Heq. now setoid_rewrite Heq. }
+    rewrite e, Genv.type_of_call_same_cp; now auto.
+    (* { unfold Genv.type_of_call; simpl in *. *)
+    (*   unfold comp_of. unfold comp_of in Heq. now setoid_rewrite Heq. } *)
     { simpl. rewrite <- comp_transf_function; eauto.
       rewrite <- (comp_transl_partial _ TTRANSF).
       eapply call_trace_lessdef; eauto using senv_preserved, symbols_preserved. }
+    (* replace (comp_of f) with (Genv.find_comp_in_genv ge (Vptr fb (Ptrofs.add ofs Ptrofs.one))). *)
+    rewrite comp_transf_function; eauto.
     econstructor; eauto.
     econstructor; eauto.
     eapply agree_sp_def; eauto.
+    (* { rewrite find_comp_translated. unfold tge. *)
+    (*   unfold Genv.find_comp_in_genv. simpl. *)
+    (*   exploit functions_transl; eauto. intros G. *)
+    (*   rewrite (Genv.find_funct_ptr_find_comp_of_block _ _ G). *)
+    (*   rewrite comp_transf_function; simpl; eauto. } *)
     { Simpl.
-      now rewrite (Genv.find_funct_ptr_find_comp_of_block _ _ CALLED). }
-    { Simpl.
-      rewrite (comp_transl_partial _ TTRANSF).
-      apply Pos.eqb_eq in Heq. rewrite <- Heq.
-      change (comp_of (Internal tf)) with (comp_of tf).
-      rewrite <- (comp_transl_partial _ H4).
-      apply match_stacks_intra_compartment. exact STACKS'.
-      unfold Mach.call_comp. simpl.
-      now rewrite (Genv.find_funct_ptr_find_comp_of_block _ _ FIND). }
-    simpl. eapply agree_exten; eauto. intros. Simpl.
-    Simpl. unfold Genv.symbol_address. rewrite symbols_preserved. rewrite H. eauto.
-    Simpl. rewrite <- H2. auto.
-  * left; econstructor; split.
-    apply plus_one. eapply exec_step_internal_call.
-    rewrite <- H2; simpl; eauto.
-    eapply functions_transl; eauto.
-    eapply find_instr_tail; eauto.
-    simpl; eauto.
-    simpl; eauto.
-    Simpl; eauto.
-    unfold Genv.symbol_address. rewrite symbols_preserved. rewrite H. eauto.
-    rewrite <- (comp_transl_partial _ H4).
-    eapply allowed_call_translated; eauto.
-    rewrite <- find_comp_of_block_translated.
-    now rewrite (Genv.find_funct_ptr_find_comp_of_block _ _ CALLED).
-    unfold update_stack_call. Simpl.
-    unfold Genv.symbol_address. rewrite symbols_preserved. rewrite H.
-    simpl; unfold tge. rewrite (Genv.find_funct_ptr_find_comp_of_block _ _ TFIND).
-    replace (comp_of tf =? comp_of tf')%positive with false.
-    rewrite <- H2. simpl. eauto. eauto.
-    { simpl. intros.
-      rewrite <- (comp_transl_partial _ H4) in H5.
-      specialize (NO_CROSS_PTR H5).
-      now eapply Val.lessdef_list_not_ptr; eauto. }
-    { simpl. rewrite <- comp_transf_function; eauto.
-      eapply call_trace_lessdef; eauto using senv_preserved, symbols_preserved. }
-    econstructor; eauto.
-    econstructor; eauto.
-    eapply agree_sp_def; eauto.
-    (* TODO: clean *)
-    { Simpl.
+      change (comp_of (Internal tf)) with (comp_of tf) in Heq.
       rewrite (Genv.find_funct_ptr_find_comp_of_block _ _ CALLED).
-      rewrite (comp_transl_partial _ TTRANSF). reflexivity. }
-    { change (comp_of (Internal tf)) with (comp_of tf) in *.
-      eapply match_stacks_cross_compartment. exact STACKS'.
-      - unfold Mach.call_comp. simpl.
-        now rewrite (Genv.find_funct_ptr_find_comp_of_block _ _ FIND).
-      - simpl.
-        rewrite <- find_comp_of_block_translated.
-        now rewrite (Genv.find_funct_ptr_find_comp_of_block _ _ FIND).
-      - rewrite (comp_transl_partial _ H4).
-        intros contra. now rewrite contra, Pos.eqb_refl in Heq.
-      - erewrite agree_sp; eauto.
-        constructor. }
+      apply match_stacks_intra_compartment; trivial.
+      replace (comp_of fd) with (comp_of f). auto.
+      { rewrite comp_transf_function; eauto.
+        unfold transf_fundef, transf_partial_fundef in TTRANSF.
+        destruct fd.
+        - monadInv TTRANSF. simpl in *.
+          rewrite comp_transf_function. rewrite e; eauto.
+          eauto.
+        - inv TTRANSF. simpl in *. auto. }
+      unfold Mach.call_comp. simpl.
+      rewrite (Genv.find_funct_ptr_find_comp_of_block _ _ FIND).
+      { simpl.
+        rewrite comp_transf_function; eauto.
+        unfold transf_fundef, transf_partial_fundef in TTRANSF.
+        destruct fd.
+        - monadInv TTRANSF. simpl in *.
+          rewrite comp_transf_function. rewrite e; eauto.
+          eauto.
+        - inv TTRANSF. simpl in *. auto. }
+    }
     simpl. eapply agree_exten; eauto. intros. Simpl.
     Simpl. unfold Genv.symbol_address. rewrite symbols_preserved. rewrite H. eauto.
     Simpl. rewrite <- H2. auto.
+    (* simpl. now rewrite (Genv.find_funct_ptr_find_comp_of_block _ _ FIND). *)
+  * destruct (flowsto_dec (comp_of tf') (comp_of tf)) eqn:?.
+    -- left; econstructor; split.
+       rewrite comp_transf_function; eauto.
+       apply plus_one. eapply exec_step_internal_call.
+       rewrite <- H2; simpl; eauto.
+       eapply functions_transl; eauto.
+       eapply find_instr_tail; eauto.
+       simpl; eauto.
+       simpl; eauto.
+       Simpl; eauto.
+       unfold Genv.symbol_address. rewrite symbols_preserved. rewrite H. eauto.
+       rewrite <- (comp_transl_partial _ H4).
+       eapply allowed_call_translated; eauto.
+       simpl.
+       now rewrite (Genv.find_funct_ptr_find_comp_of_block _ _ TFIND).
+       unfold update_stack_call. Simpl.
+       (* rewrite H7; simpl. *)
+       (* simpl. *)
+       unfold Genv.symbol_address. rewrite symbols_preserved. rewrite H. simpl.
+       unfold tge; rewrite (Genv.find_funct_ptr_find_comp_of_block _ _ TFIND).
+       rewrite <- H2. simpl. rewrite Heq.
+       reflexivity.
+       eauto.
+       { simpl.
+         intros.
+         rewrite <- (comp_transl_partial _ H4) in H5.
+         rewrite <- (comp_transl_partial _ TTRANSF) in H5.
+         specialize (NO_CROSS_PTR H5).
+         now eapply Val.lessdef_list_not_ptr; eauto. }
+       { simpl. rewrite <- comp_transf_function; eauto.
+         rewrite <- (comp_transl_partial _ TTRANSF).
+         eapply call_trace_lessdef; eauto using senv_preserved, symbols_preserved. }
+       (* replace (comp_of f) *)
+       (*   with (Genv.find_comp_in_genv ge (Vptr fb (Ptrofs.add ofs Ptrofs.one))). *)
+       rewrite comp_transf_function; eauto.
+       econstructor; eauto.
+       econstructor; eauto.
+       eapply agree_sp_def; eauto.
+       (* TODO: clean *)
+       { eapply match_stacks_cross_compartment. exact STACKS'.
+         - unfold Mach.call_comp. simpl.
+           now rewrite (Genv.find_funct_ptr_find_comp_of_block _ _ FIND).
+         - simpl.
+           rewrite <- find_comp_of_block_translated.
+           now rewrite (Genv.find_funct_ptr_find_comp_of_block _ _ H3).
+         - rewrite (Genv.find_funct_ptr_find_comp_of_block _ _ CALLED).
+           simpl.
+           rewrite comp_transf_function; eauto.
+           unfold transf_fundef, transf_partial_fundef in TTRANSF.
+           destruct fd.
+           + monadInv TTRANSF. simpl in *.
+             rewrite comp_transf_function; eauto.
+           + inv TTRANSF. simpl in *. auto.
+         - erewrite agree_sp; eauto.
+           constructor.
+       }
+       simpl. eapply agree_exten; eauto. intros. Simpl.
+       unfold Genv.symbol_address. rewrite symbols_preserved. rewrite H. simpl.
+       Simpl. rewrite <- H2. auto.
+       (* simpl. *)
+       (* now rewrite (Genv.find_funct_ptr_find_comp_of_block _ _ H3). *)
+    -- left; econstructor; split.
+       rewrite comp_transf_function; eauto.
+       apply plus_one. eapply exec_step_internal_call.
+       rewrite <- H2; simpl; eauto.
+       eapply functions_transl; eauto.
+       eapply find_instr_tail; eauto.
+       simpl; eauto.
+       simpl; eauto.
+       Simpl; eauto.
+       unfold Genv.symbol_address. rewrite symbols_preserved. rewrite H. auto.
+       rewrite <- (comp_transl_partial _ H4).
+       eapply allowed_call_translated; eauto.
+       simpl.
+       now rewrite (Genv.find_funct_ptr_find_comp_of_block _ _ TFIND).
+       unfold update_stack_call. Simpl.
+       unfold Genv.symbol_address. rewrite symbols_preserved. rewrite H. simpl.
+       unfold tge; rewrite (Genv.find_funct_ptr_find_comp_of_block _ _ TFIND).
+       rewrite <- H2. simpl. rewrite Heq.
+       reflexivity.
+       eauto.
+       { simpl.
+         intros.
+         rewrite <- (comp_transl_partial _ H4) in H5.
+         rewrite <- (comp_transl_partial _ TTRANSF) in H5.
+         specialize (NO_CROSS_PTR H5).
+         now eapply Val.lessdef_list_not_ptr; eauto. }
+       { simpl. rewrite <- comp_transf_function; eauto.
+         rewrite <- (comp_transl_partial _ TTRANSF).
+         eapply call_trace_lessdef; eauto using senv_preserved, symbols_preserved. }
+       (* replace (comp_of f) *)
+       (*   with (Genv.find_comp_in_genv ge (Vptr fb (Ptrofs.add ofs Ptrofs.one))). *)
+       rewrite comp_transf_function; eauto.
+       econstructor; eauto.
+       econstructor; eauto.
+       eapply agree_sp_def; eauto.
+       (* { rewrite find_comp_translated. unfold tge. *)
+       (*   unfold Genv.find_comp_in_genv. simpl. *)
+       (*   exploit functions_transl; eauto. intros G. *)
+       (*   rewrite (Genv.find_funct_ptr_find_comp_of_block _ _ G). *)
+       (*   rewrite comp_transf_function; simpl; eauto. } *)
+       (* TODO: clean *)
+       { eapply match_stacks_cross_compartment. exact STACKS'.
+         - unfold Mach.call_comp. simpl.
+           now rewrite (Genv.find_funct_ptr_find_comp_of_block _ _ FIND).
+         - simpl.
+           rewrite <- find_comp_of_block_translated.
+           now rewrite (Genv.find_funct_ptr_find_comp_of_block _ _ H3).
+         (* - rewrite (comp_transl_partial _ TTRANSF). *)
+         (*   rewrite (comp_transl_partial _ H4). *)
+         (*   intros contra. now rewrite contra, Pos.eqb_refl in Heq. *)
+         - rewrite (Genv.find_funct_ptr_find_comp_of_block _ _ CALLED).
+           simpl.
+           rewrite comp_transf_function; eauto.
+           unfold transf_fundef, transf_partial_fundef in TTRANSF.
+           destruct fd.
+           + monadInv TTRANSF. simpl in *.
+             rewrite comp_transf_function; eauto.
+           + inv TTRANSF. simpl in *. auto.
+         - erewrite agree_sp; eauto.
+           constructor.
+       }
+       simpl. eapply agree_exten; eauto. intros. Simpl.
+       unfold Genv.symbol_address. rewrite symbols_preserved. rewrite H. simpl.
+       Simpl. rewrite <- H2. auto.
+       (* simpl. now rewrite (Genv.find_funct_ptr_find_comp_of_block _ _ H3). *)
 
 - (* Mtailcall *)
   assert (f0 = f) by congruence.  subst f0.
@@ -1075,6 +1295,8 @@ Local Transparent destroyed_by_op.
   left; econstructor; split.
   (* execution *)
   eapply plus_right'. eapply exec_straight_exec; eauto.
+  now rewrite <- H4; simpl; erewrite Genv.find_funct_ptr_find_comp_of_block; eauto.
+  rewrite comp_transf_function; eauto.
   econstructor. eexact P. eapply functions_transl; eauto. eapply find_instr_tail. eexact Q.
   reflexivity.
   simpl. reflexivity. eauto. eauto.
@@ -1084,6 +1306,7 @@ Local Transparent destroyed_by_op.
   now rewrite <- find_comp_of_block_translated, NEXTCOMP.
   traceEq.
   (* match states *)
+  rewrite comp_transf_function; eauto.
   econstructor; eauto.
   apply agree_set_other; auto with asmgen.
   Simpl. rewrite Z by (rewrite <- (ireg_of_eq _ _ EQ1); eauto with asmgen). assumption.
@@ -1094,7 +1317,10 @@ Local Transparent destroyed_by_op.
   intros (ofs' & P & Q).
   left; econstructor; split.
   (* execution *)
+  rewrite comp_transf_function; eauto.
   eapply plus_right'. eapply exec_straight_exec; eauto.
+  rewrite <- comp_transf_function; eauto.
+  now rewrite <- H4; simpl; erewrite Genv.find_funct_ptr_find_comp_of_block; eauto.
   econstructor. eexact P. eapply functions_transl; eauto. eapply find_instr_tail. eexact Q.
   reflexivity.
   simpl. reflexivity. eauto. eauto.
@@ -1104,6 +1330,7 @@ Local Transparent destroyed_by_op.
   simpl. now rewrite <- find_comp_of_block_translated.
   traceEq.
   (* match states *)
+  rewrite comp_transf_function; eauto.
   econstructor; eauto.
   apply agree_set_other; auto with asmgen.
   apply agree_set_other; auto with asmgen.
@@ -1117,14 +1344,18 @@ Local Transparent destroyed_by_op.
   exploit external_call_mem_extends; eauto.
   intros [vres' [m2' [A [B [C D]]]]].
   left. econstructor; split. apply plus_one.
+  rewrite comp_transf_function; eauto.
   eapply exec_step_builtin. eauto. eauto.
   eapply find_instr_tail; eauto.
   erewrite <- sp_val by eauto.
   eapply eval_builtin_args_preserved with (ge1 := ge); eauto. exact symbols_preserved.
-  eapply external_call_symbols_preserved; eauto. apply senv_preserved.
   rewrite <- (comp_transl_partial _ H3).
-  unfold_find_comp CURCOMP FIND. rewrite <- CURCOMP. reflexivity.
+  erewrite Genv.find_funct_ptr_find_comp_of_block in A; eauto. simpl in A.
+  eapply external_call_symbols_preserved; eauto. apply senv_preserved.
+  (* rewrite <- (comp_transl_partial _ H3). *)
+  (* unfold_find_comp_in_genv CURCOMP FIND. rewrite <- CURCOMP. reflexivity. *)
   eauto.
+  rewrite <- comp_transf_function; eauto.
   econstructor; eauto.
   instantiate (2 := tf); instantiate (1 := x).
   unfold nextinstr. rewrite Pregmap.gss.
@@ -1144,11 +1375,12 @@ Local Transparent destroyed_by_op.
   inv AT. monadInv H4.
   exploit find_label_goto_label; eauto. intros [tc' [rs' [GOTO [AT2 INV]]]].
   exploit functions_transl; eauto. intro FN.
-  left. inversion AT2; subst. exists (State s' rs' m'); split.
+  left. inversion AT2; subst.
+  exists (State s' rs' m' (comp_of f)); split.
+  rewrite comp_transf_function; eauto.
   apply plus_one. econstructor; eauto.
   eapply find_instr_tail; eauto.
   simpl; eauto. eauto. eauto.
-  simpl; unfold Genv.find_comp; simpl.
   now rewrite (Genv.find_funct_ptr_find_comp_of_block _ _ FN).
   econstructor; eauto.
   eapply agree_exten; eauto with asmgen.
@@ -1195,13 +1427,14 @@ Local Transparent destroyed_by_op.
   simpl. rewrite <- H9. unfold Mach.label in H0; unfold label; rewrite H0.
   eexact A. eauto. eauto. eauto.
   simpl.
-  simpl; unfold Genv.find_comp; simpl.
+  (* simpl; unfold Genv.find_comp; simpl. *)
   now rewrite (Genv.find_funct_ptr_find_comp_of_block _ _ FN).
 
   assert (exists ofs, rs' PC = Vptr fb ofs) as [ofs' Hptr]. {
     destruct (rs' PC); inversion B.
     eauto.
   }
+  rewrite <- comp_transf_function; eauto.
   econstructor; eauto.
   eapply agree_undef_regs; eauto.
   simpl. intros. rewrite C; auto with asmgen. Simpl.
@@ -1220,6 +1453,7 @@ Local Transparent destroyed_by_op.
   left; econstructor; split.
   eapply plus_star_trans.
   eapply exec_straight_exec; eauto.
+  now rewrite <- H3; simpl; erewrite Genv.find_funct_ptr_find_comp_of_block; eauto.
   eapply star_step. eapply exec_step_internal_return; eauto.
   eapply functions_transl; eauto. eapply find_instr_tail. eexact Q.
   simpl. reflexivity. eauto.
@@ -1277,7 +1511,8 @@ Local Transparent destroyed_by_op.
   left; eexists; split.
   eapply exec_straight_steps_1; eauto. lia. simpl. constructor.
   econstructor; eauto.
-  unfold_find_comp STACKS_COMP H. now subst cp.
+  erewrite Genv.find_funct_ptr_find_comp_of_block in STACKS'; eauto. now simpl in STACKS'.
+  (* unfold_find_comp_in_genv STACKS_COMP H. now subst cp. *)
   rewrite X; econstructor; eauto.
   apply agree_exten with rs2; eauto with asmgen.
   unfold rs2.
@@ -1305,9 +1540,10 @@ Local Transparent destroyed_at_function_entry.
   left; econstructor; split.
   apply plus_one. eapply exec_step_external; eauto.
   eapply external_call_symbols_preserved; eauto. apply senv_preserved.
-  unfold_find_comp STACKS_COMP H. subst cp.
+  (* unfold_find_comp_in_genv STACKS_COMP H. subst cp. *)
   econstructor; eauto.
-  Simpl. rewrite ATLR. eauto.
+  erewrite Genv.find_funct_ptr_find_comp_of_block in STACKS'; eauto. simpl in STACKS'. auto.
+  (* Simpl. rewrite ATLR. eauto. *)
   eapply agree_set_other; eauto.
   eapply agree_set_pair; eauto. eapply agree_undef_caller_save_regs; eauto.
 
@@ -1319,25 +1555,25 @@ Local Transparent destroyed_at_function_entry.
     rewrite <- find_comp_of_block_translated.
     rewrite (Genv.find_funct_ptr_find_comp_of_block _ _ H3).
     change (comp_of (Internal f0)) with (comp_of f0).
-    destruct (cp =? comp_of f0)%positive eqn:e.
-    - apply Pos.eqb_eq in e. subst cp.
+    destruct (cp_eq_dec cp (comp_of f0)) eqn:e.
+    - subst cp.
+      (* apply Pos.eqb_eq in e. subst cp. *)
       eexists; split; auto.
       inv STACKS'; auto.
       unfold Mach.call_comp in *; simpl in *.
-      rewrite (Genv.find_funct_ptr_find_comp_of_block _ _ H3) in H2.
-      change (comp_of (Internal f0)) with (comp_of f0) in *.
-      congruence.
+      rewrite (Genv.find_funct_ptr_find_comp_of_block _ _ H3) in H4.
+      simpl in *.
+      inv H10.
+      rewrite find_comp_of_block_translated in H5. congruence.
     - inv STACKS'; auto.
       + unfold Mach.call_comp in *. simpl in *.
-        rewrite (Genv.find_funct_ptr_find_comp_of_block _ _ H3) in H4.
-        injection H4 as E. subst cp.
-        now rewrite Pos.eqb_refl in e.
+        clear e.
+        rewrite (Genv.find_funct_ptr_find_comp_of_block _ _ H3) in n. simpl in n.
+        congruence.
       + unfold Mach.call_comp in *. simpl in *.
-        rewrite (Genv.find_funct_ptr_find_comp_of_block _ _ H3) in H2.
-        injection H2 as E. subst cp'0. eauto.
-  }
+        rewrite (Genv.find_funct_ptr_find_comp_of_block _ _ H3) in H1. eauto. }
 
-  left. eexists (State s'' rs0 m'). split.
+  left. eexists (State s'' rs0 m' (comp_of f0)). split.
   assert (LD: Val.lessdef (Mach.return_value rs sg) (return_value rs0 sg)).
   { unfold Mach.return_value, return_value.
     destruct (loc_result sg).
@@ -1349,40 +1585,35 @@ Local Transparent destroyed_at_function_entry.
   econstructor; eauto.
   rewrite ATPC. unfold Vnullptr. now destruct Archi.ptr64.
   { rewrite ATPC. simpl. rewrite <- find_comp_of_block_translated.
-    eauto. }
+    now erewrite (Genv.find_funct_ptr_find_comp_of_block); eauto. }
   { rewrite ATPC. simpl.
     intros diff.
     inv STACKS'; auto.
-    - simpl in *. subst. unfold Mach.call_comp in *. simpl in *. congruence.
+    - simpl in diff. erewrite Genv.find_funct_ptr_find_comp_of_block in diff; eauto. now simpl in diff.
     - inv H10. reflexivity. }
   { intros diff.
     inv STACKS'; auto.
-    - simpl in *. subst. unfold Mach.call_comp in *. simpl in *.
-      congruence.
+    - simpl in diff. erewrite Genv.find_funct_ptr_find_comp_of_block in diff; eauto. now simpl in diff.
     - inv H10. eapply agree_sp; eauto. }
   { intros TYPE.
     inv STACKS'; auto.
-    - simpl in *. subst. unfold Mach.call_comp in *. simpl in *.
-      assert (cp' = cp) by congruence. subst cp'.
-      now eapply Genv.type_of_call_same_cp in TYPE.
-    - simpl in *. subst. unfold Mach.call_comp in *. simpl in *.
-      inv H10.
+    - simpl in *. erewrite Genv.find_funct_ptr_find_comp_of_block in TYPE; eauto. simpl in TYPE.
+      pose proof (flowsto_refl (comp_of f0)); now destruct (flowsto_dec (comp_of f0) (comp_of f0)).
+    - simpl in *. erewrite Genv.find_funct_ptr_find_comp_of_block in NO_CROSS_PTR; eauto. simpl in *.
       specialize (NO_CROSS_PTR TYPE).
+      inv H10.
       (* TODO: factorize into a lemma Val.lessdef_not_ptr *)
       inv LD; auto. now rewrite <- H0 in NO_CROSS_PTR. }
   { inv STACKS'; auto.
-    - simpl in *. subst. unfold Mach.call_comp in *. simpl in *.
-      rewrite (Genv.find_funct_ptr_find_comp_of_block _ _ H3) in H4.
-      change (comp_of (Internal f0)) with (comp_of f0) in *.
-      injection H4 as <-.
-      rewrite (Genv.find_funct_ptr_find_comp_of_block _ _ H3) in CURCOMP.
-      injection CURCOMP as <-.
+    - simpl in *.
+      rewrite (Genv.find_funct_ptr_find_comp_of_block _ _ H3) in *. simpl in *.
       assert (t = E0).
-      { inv EV; auto.
-        exfalso. eapply Genv.type_of_call_same_cp. eauto. }
-      subst. constructor. now apply Genv.type_of_call_same_cp.
-    - simpl in *. unfold Mach.call_comp in *. simpl in *.
-      inv H10.
+      { inv EV; auto. rewrite Genv.type_of_call_same_cp in H; now auto. }
+      subst.
+      constructor.
+      rewrite Genv.type_of_call_same_cp; now auto.
+    - simpl in *. inv H10.
+      erewrite Genv.find_funct_ptr_find_comp_of_block in EV; eauto.
       eapply return_trace_lessdef with (ge := ge) (v := Mach.return_value rs sg);
         eauto using senv_preserved. }
 
